theories/TypeSystem.v
@@ -15,22 +15,24 @@ Require Import Local.Metatheory.
 Definition env: Set :=
   list pseudoterm.
 
-(* We are free to take a simpler definition here since there are no dependent
-   types. We skip several lifting operations on purpose. *)
+Inductive simple: pseudoterm -> Prop :=
+  | simple_base:
+    simple base
+  | simple_negation:
+    forall ts,
+    Forall simple ts -> simple (negation ts).
+
+Definition valid_env (g: env): Prop :=
+  Forall simple g.
+
+(* We are free to take a simpler definition here since we're only dealing with
+   simple types. Reasoning about dependent types will require extra care! *)
 
 Inductive typing: env -> relation pseudoterm :=
-  | typing_base:
-    forall g,
-    valid_env g -> typing g base prop
-  | typing_negation:
-    forall g ts,
-    Forall (fun t => typing g t prop) ts ->
-    valid_env g ->
-    typing g (negation ts) prop
   | typing_bound:
     forall g n t,
-    item t g n ->
     valid_env g ->
+    item t g n ->
     typing g n t
   | typing_jump:
     forall g k xs ts,
@@ -39,401 +41,33 @@ Inductive typing: env -> relation pseudoterm :=
     typing g (jump k xs) void
   | typing_bind:
     forall g b ts c,
-    typing (negation ts :: g) b void ->
-    Forall (fun t => typing g t prop) ts ->
     typing (ts ++ g) c void ->
-    typing g (bind b ts c) void
-
-with valid_env: env -> Prop :=
-  | valid_env_nil:
-    valid_env []
-  | valid_env_term_var:
-    forall g t,
-    typing g t prop -> valid_env (t :: g).
+    typing (negation ts :: g) b void ->
+    typing g (bind b ts c) void.
 
 Global Hint Constructors typing: cps.
-Global Hint Constructors valid_env: cps.
 
-Lemma valid_env_typing:
-  forall g e t,
-  typing g e t -> valid_env g.
-Proof.
-  induction 1.
-  - assumption.
-  - assumption.
-  - assumption.
-  - assumption.
-  - dependent destruction IHtyping1.
-    dependent destruction H2.
-    assumption.
-Qed.
-
-Global Hint Resolve valid_env_typing: cps.
-
-Lemma valid_env_inv:
-  forall x g,
-  valid_env (x :: g) -> valid_env g.
+Lemma typing_bound_is_simple:
+  forall g n t,
+  typing g (bound n) t ->
+  simple t.
 Proof.
   intros.
   dependent destruction H.
-  apply valid_env_typing with x prop; auto.
-Qed.
-
-Global Hint Resolve valid_env_inv: cps.
-
-Lemma typing_deepind:
-  forall P: (forall g e t, Prop),
-  forall f1: (forall g,
-              valid_env g -> P g base prop),
-  forall f2: (forall g ts,
-              valid_env g ->
-              Forall (fun t => typing g t prop) ts ->
-              Forall (fun t => P g t prop) ts ->
-              P g (negation ts) prop),
-  forall f3: (forall g n t,
-              valid_env g ->
-              item t g n ->
-              P g n t),
-  forall f4: (forall g k xs ts,
-              typing g k (negation ts) ->
-              Forall2 (typing g) (rev xs) ts ->
-              P g k (negation ts) ->
-              Forall2 (P g) (rev xs) ts ->
-              P g (jump k xs) void),
-  forall f5: (forall g b ts c,
-              typing (negation ts :: g) b void ->
-              Forall (fun t => typing g t prop) ts ->
-              typing (ts ++ g) c void ->
-              P (negation ts :: g) b void ->
-              Forall (fun t => P g t prop) ts ->
-              P (ts ++ g) c void ->
-              P g (bind b ts c) void),
-  forall g e t,
-  typing g e t -> P g e t.
-Proof.
-  do 6 intro; fix H 4.
-  destruct 1.
-  - apply f1; auto.
-  - apply f2; auto.
-    clear f1 f2 f3 f4 f5 H1.
-    induction H0; auto.
-  - apply f3; auto.
-  - apply f4 with ts; auto.
-    clear f1 f2 f3 f4 f5 H0.
-    induction H1; auto.
-  - apply f5; auto.
-    clear f1 f2 f3 f4 f5 H0_ H0_0.
-    induction H0; auto.
+  replace t with (nth n g void).
+  - apply Forall_nth.
+    + assumption.
+    + apply item_valid_index with t.
+      assumption.
+  - apply nth_item.
+    assumption.
 Qed.
 
 Lemma typing_bound_cant_be_void:
   forall g n,
   ~typing g (bound n) void.
 Proof.
-  intros g n H.
-  dependent destruction H.
-  induction H.
-  - dependent destruction H0.
-    inversion H.
-  - dependent destruction H0.
-    eauto with cps.
-Qed.
-
-Lemma typing_bound_cant_be_prop:
-  forall g n,
-  ~typing g (bound n) prop.
-Proof.
-  intros g n H.
-  dependent destruction H.
-  induction H.
-  - dependent destruction H0.
-    inversion H.
-  - dependent destruction H0.
-    eauto with cps.
-Qed.
-
-Lemma typing_type_lift_inversion:
-  forall g t,
-  typing g t prop ->
-  forall i k,
-  lift i k t = t.
-Proof.
-  intros until 1.
-  dependent induction H using typing_deepind; intros.
-  - reflexivity.
-  - clear H0.
-    rewrite lift_distributes_over_negation; f_equal.
-    induction H1; simpl.
-    + reflexivity.
-    + f_equal; auto.
-  - absurd (typing g n prop).
-    + apply typing_bound_cant_be_prop.
-    + constructor; auto.
-Qed.
-
-Local Hint Resolve typing_type_lift_inversion: cps.
-
-Lemma typing_type_list_lift_inversion:
-  forall ts g,
-  Forall (fun t : pseudoterm => typing g t prop) ts ->
-  forall i k,
-  traverse_list (lift i) k ts = ts.
-Proof.
-  induction 1; simpl; intros.
-  - reflexivity.
-  - f_equal; eauto with cps.
-Qed.
-
-Local Hint Resolve typing_type_list_lift_inversion: cps.
-
-Lemma typing_type_unlift:
-  forall g t i k,
-  typing g (lift i k t) prop ->
-  typing g t prop.
-Proof.
-  intros.
-  dependent induction H using typing_deepind.
-  - destruct t; try discriminate.
-    + constructor; auto.
-    + exfalso.
-      destruct (le_gt_dec k n).
-      * rewrite lift_bound_ge in x; auto.
-        discriminate.
-      * rewrite lift_bound_lt in x; auto.
-        discriminate.
-  - destruct t; try discriminate.
-    + exfalso.
-      destruct (le_gt_dec k n).
-      * rewrite lift_bound_ge in x; auto.
-        discriminate.
-      * rewrite lift_bound_lt in x; auto.
-        discriminate.
-    + clear H0.
-      dependent destruction x.
-      constructor; auto.
-      dependent induction H1.
-      * destruct ts0; try discriminate.
-        constructor.
-      * destruct ts0; try discriminate.
-        dependent destruction x.
-        constructor; eauto.
-        eapply H0; auto.
-        reflexivity.
-  - absurd (typing g n prop).
-    + apply typing_bound_cant_be_prop.
-    + constructor; auto.
-Qed.
-
-Lemma typing_type_preserved_under_any_env:
-  forall g t,
-  typing g t prop ->
-  forall h,
-  valid_env h ->
-  typing h t prop.
-Proof.
-  intros until 1.
-  dependent induction H using typing_deepind; intros.
-  - constructor; auto.
-  - clear H H0.
-    constructor; auto.
-    induction H1; simpl.
-    + constructor.
-    + constructor; auto.
-  - absurd (typing g n prop).
-    + apply typing_bound_cant_be_prop.
-    + constructor; auto.
-Qed.
-
-Local Hint Resolve typing_type_preserved_under_any_env: cps.
-
-Lemma typing_negation_inversion:
-  forall g k ts,
-  typing g k (negation ts) ->
-  forall h,
-  valid_env h ->
-  Forall (fun t => typing h t prop) ts.
-Proof.
-  intros until 1.
-  dependent destruction H.
-  dependent induction H; intros.
-  - dependent destruction H0.
-    dependent destruction H.
-    induction H; simpl.
-    + constructor.
-    + constructor; auto.
-      eapply typing_type_preserved_under_any_env; eauto.
-  - apply IHitem; auto.
-    eapply valid_env_inv; eauto.
-Qed.
-
-Lemma typing_bound_has_type:
-  forall t g n,
-  item t g n ->
-  valid_env g ->
-  forall h,
-  valid_env h -> typing h t prop.
-Proof.
-  induction 1; intros.
-  - dependent destruction H.
-    eapply typing_type_preserved_under_any_env; eauto.
-  - apply IHitem; auto.
-    eapply valid_env_inv.
-    eassumption.
-Qed.
-
-(* -------------------------------------------------------------------------- *)
-
-(* TODO: move this to Prelude. *)
-
-Inductive insert item: nat -> relation env :=
-  | insert_head:
-    forall tail,
-    insert item 0 tail (item :: tail)
-  | insert_tail:
-    forall k head tail1 tail2,
-    insert item k tail1 tail2 ->
-    insert item (S k) (head :: tail1) (head :: tail2).
-
-Global Hint Constructors insert: cps.
-
-Lemma insert_bound_ge:
-  forall x n g h,
-  insert x n g h ->
-  forall m,
-  n <= m ->
-  forall y,
-  item y g m -> item y h (S m).
-Proof.
-  induction 1; intros.
-  - auto with cps.
-  - destruct m.
-    + exfalso.
-      inversion H0.
-    + dependent destruction H1.
-      auto with arith cps.
-Qed.
-
-Lemma insert_bound_lt:
-  forall e n g h,
-  insert e n g h ->
-  forall m,
-  n > m ->
-  forall t,
-  item t g m -> item t h m.
-Proof.
-  induction 1; intros.
-  - inversion H.
-  - destruct m.
-    + dependent destruction H1.
-      constructor.
-    + dependent destruction H1.
-      constructor.
-      apply IHinsert; auto.
-      lia.
-Qed.
-
-Lemma insert_app_tail:
-  forall x n ts g h,
-  insert x n g h ->
-  insert x (n + length ts) (ts ++ g) (ts ++ h).
-Proof.
-  induction ts; simpl; intros.
-  - rewrite Nat.add_0_r.
-    assumption.
-  - rewrite Nat.add_succ_r; simpl.
-    constructor; auto.
-Qed.
-
-Local Hint Resolve insert_app_tail: cps.
-
-(** ** Weakening *)
-
-Lemma typing_weak_lift:
-  forall g e t,
-  typing g e t ->
-  forall x n h,
-  insert x n g h ->
-  valid_env h ->
-  typing h (lift 1 n e) t.
-Proof.
-  intros until 1.
-  induction H using typing_deepind; intros.
-  - auto with cps.
-  - rewrite lift_distributes_over_negation.
-    erewrite typing_type_list_lift_inversion; eauto.
-    apply typing_negation; auto.
-    clear H0.
-    induction H1.
-    + constructor.
-    + constructor; auto.
-      apply typing_type_unlift with 1 n; eauto.
-  - rename n0 into k.
-    destruct (le_gt_dec k n).
-    + rewrite lift_bound_ge; auto.
-      constructor; auto.
-      apply insert_bound_ge with x k g; auto.
-    + rewrite lift_bound_lt; auto.
-      constructor; auto.
-      apply insert_bound_lt with x k g; auto.
-  - rewrite lift_distributes_over_jump.
-    apply typing_jump with ts.
-    + apply IHtyping with x; auto.
-    + clear IHtyping H H0.
-      rewrite <- map_rev.
-      generalize dependent (rev xs); intros ys ?.
-      induction H1; simpl.
-      * constructor.
-      * constructor; eauto.
-  - rewrite lift_distributes_over_bind.
-    apply typing_bind.
-    + rewrite typing_type_list_lift_inversion with (g := h).
-      * apply valid_env_typing in H.
-        dependent destruction H.
-        apply IHtyping1 with x; eauto with cps.
-      * clear H H1 H2 IHtyping1 IHtyping2.
-        induction H0; eauto with cps.
-    + erewrite typing_type_list_lift_inversion; eauto.
-      clear H H1 H2 H3 IHtyping1 IHtyping2.
-      induction H0.
-      * constructor.
-      * constructor; auto.
-        apply typing_type_preserved_under_any_env with g; auto.
-    + rewrite typing_type_list_lift_inversion with (g := h).
-      * apply valid_env_typing in H1.
-        apply IHtyping2 with x; auto with cps.
-        (* We could use a simpler solution, but let's build it grounds up. *)
-        clear H H0 H1 IHtyping1 IHtyping2.
-        induction H2; simpl; auto.
-        constructor.
-        apply typing_type_unlift with 1 n; eauto with cps.
-      * clear H H1 H2 IHtyping1 IHtyping2.
-        induction H0; eauto with cps.
-Qed.
-
-Theorem weakening:
-  forall g e t,
-  typing g e t ->
-  forall x,
-  valid_env (x :: g) ->
-  typing (x :: g) (lift 1 0 e) t.
-Proof.
-  intros.
-  eapply typing_weak_lift; eauto with cps.
-Qed.
-
-Corollary typing_lift:
-  forall g e t,
-  typing g e t ->
-  forall h,
-  valid_env (h ++ g) ->
-  typing (h ++ g) (lift (length h) 0 e) t.
-Proof.
-  induction h; simpl; intros.
-  - rewrite lift_zero_e_equals_e.
-    assumption.
-  - rewrite <- lift_lift_simplification with (i := 1) (k := 0) (e := e);
-      try lia.
-    apply weakening; auto.
-    apply IHh.
-    eapply valid_env_inv; eauto.
+  intros g n ?.
+  apply typing_bound_is_simple in H.
+  inversion H.
 Qed.
