theories/Prelude.v
@@ -188,6 +188,12 @@ Proof.
   induction 1; simpl; lia.
 Qed.
 
+Section Lists.
+
+
+
+End Lists.
+
 Section SetoidFix.
 
   (* The code in this section is taken from coq-ext-lib and slightly adapted;
